src/Find_proof_3.thy
@@ -1,11 +1,89 @@
-theory Find_proof_3 imports Find_tree_stack begin
+theory 
+Find_proof_3 imports 
+Find_tree_stack begin
 
-lemma invariant_wf_fts_lem: "invariant_wf_fts_lem"
-sorry
-
-definition guard :: "'a \<Rightarrow> 'a" where "guard a = a"
-
-lemma map_comp: "map (f o g) xs = map f (map g xs)" apply(force) done
+lemma invariant_wf_fts: "invariant_wf_fts_lem"
+apply(simp add: invariant_wf_fts_lem_def)
+apply(simp add: invariant_def)
+apply(intro allI impI)
+apply(rename_tac f ts f' ts')
+apply(simp add: fts_trans_def)
+apply(subgoal_tac "? k xs l t u zs. f|>dest_fts_focus|>dest_core = (k,xs,l,t,u,zs)") prefer 2 apply(force intro:FIXME)
+apply(elim exE)
+apply(subgoal_tac "k=k0") prefer 2 apply(force intro: FIXME)
+apply(subgoal_tac "(? kvs. t = Leaf kvs) | (? ks rs. (t = Node(ks,rs)))") prefer 2 apply(force intro:FIXME)
+apply(erule disjE)
+ (* Leaf *)
+ apply(elim exE)
+ apply(force simp add: step_fts_def)
+(* Node(ks,rs) *)
+apply(elim exE)
+(* unfolding of step_fts let bindings *)
+apply(subgoal_tac "
+   (?  i.  (search_key_to_index ks k = i) &
+   (? cn. ((
+      let core = mk_core (k,xs,l,t,u,zs) in
+      let ksrsi = (| cc_ks=ks,cc_rs=rs,cc_i=i |) in
+      (core,ksrsi)) = cn) &
+    (? ts2. ((cn # ts) = ts2)) &
+    (* new focus ----- *)
+    (? isx isy. ((from_to 0 (i-1), i, from_to (i+1) (ks_to_max_child_index ks)) = (isx,i,isy)) &
+    (? tsx t2 tsy. ((indexes_to_trees rs isx, rs!i, indexes_to_trees rs isy) = (tsx,t2,tsy)) & 
+    (? xs' zs'. (
+      (tsx |> List.map tree_to_leaves |> List.concat, tsy |> List.map tree_to_leaves |> List.concat) = (xs',zs'))
+    &  
+    (? l2 u2. cnode_to_bound cn  = (l2,u2)))))))
+  ") prefer 2 apply(force)
+apply(elim exE conjE)
+apply(simp add: step_fts_def)
+apply(elim conjE)
+apply(drule_tac t = ts' in sym)
+apply(simp)
+apply(simp (no_asm) add: wellformed_fts_def)
+apply(intro conjI)
+ (* 3 subgs *)
+ (* wf_ts ts' *)
+ apply(simp add: wellformed_ts_def_2)
+ apply(intro conjI)
+  (* wf_cnode *)
+  apply(drule_tac t=cn in sym)
+  apply(simp)
+  apply(simp add: wellformed_cnode_def)
+  (* wf_core f *)
+  (* should follow from wf_fts *)
+  apply(simp add: wellformed_fts_def)
+  apply(simp add: wellformed_fts_focus_def)
+  apply(force simp add: wellformed_core_def)
+   
+  (* wf_ts ts*)
+  (* from wf_fts *)
+  apply(force simp add: wellformed_fts_def)
+   
+ (* wf_fts_focus f' *)
+ apply(drule_tac t=f' in sym)
+ apply(simp)
+ apply(simp add: wellformed_fts_focus_def)
+ (* wf_core f' *)
+ apply(simp add: wellformed_core_def)
+ apply(intro conjI)
+  (* wf_tree t2 *)
+  (* ts = rs ! i, and use wf_focus f *)
+  apply(simp add: wellformed_fts_def) apply(elim conjE)
+  apply(simp add: wellformed_fts_focus_def)
+  apply(simp add: wellformed_core_def)
+  (* now have wf_tree Node(ks,rs) *)
+  apply(force intro: FIXME )
+  
+  (* ck2 xs@xs' etc; the difficult part *)
+  apply(force intro: FIXME)
+  
+ (* wellformed_fts_1 f' *)
+ apply(simp add: wellformed_fts_1_def)
+ apply(drule_tac t=cn in sym)
+ apply(simp)
+ apply(drule_tac t=f' in sym)
+ apply(force)
+done
 
 lemma lem_2: "! P Q.
 ((% fts. wellformed_fts k0 fts) = P) \<longrightarrow>
